CFGdef.v
@@ -1,0 +1,214 @@
+Set Nested Proofs Allowed.
+
+Require Export Coq.Logic.Decidable.
+Require Export Coq.Classes.EquivDec.
+Require Export Coq.Bool.Bool.
+Require Export Lists.List.
+Require Export Coq.Program.Equality.
+Require Export Coq.Program.Utils.
+
+(*Require Import finiteTypes.External.
+Require Import finiteTypes.BasicDefinitions.*)
+
+Require Export FinTypes.
+
+Require Export Graph SimplDec.
+
+(*  Notation "p '-->*' q" := (exists π, Path p q π) (at level 55, right associativity).*)
+
+(** Definition of the reducible CFG **)
+
+Reserved Infix "-->b" (at level 55).
+Reserved Infix "-a>" (at level 55).
+Reserved Infix "-a>*" (at level 55).
+
+Class redCFG
+      (Lab : finType)
+      (edge : Lab -> Lab -> bool)
+      (root : Lab) 
+      (a_edge : Lab -> Lab -> bool)
+  :=
+    {
+      back_edge_b := minus_edge edge a_edge
+                     where "p -->b q" := (edge p q);
+      back_edge := (fun p q => back_edge_b p q = true)
+                   where "p --> q"  := (p -->b q = true);
+      (* reducibility *)
+      loop_head_dom : forall ql qh, back_edge ql qh -> Dom edge root qh ql
+      where "p -a> q" := (a_edge p q = true);
+      a_edge_incl : sub_graph a_edge edge
+      where "p '-a>*' q" := (exists π, Path a_edge p q π);
+      a_edge_acyclic : acyclic a_edge;
+      a_reachability : forall q, (exists π, Path a_edge root q π);
+      (* useful definitions *)
+      loop_head h := exists p, back_edge p h;
+      loop_contains qh q := exists p π, back_edge p qh /\ Path edge q p π /\ qh ∉ tl (rev π);
+      exit_edge h p q := loop_contains h p /\ ~ loop_contains h q /\ p --> q;
+      (* the following restrictions can be easily be met by introducing new blocks *)
+      single_exit : forall h p q, exit_edge h p q -> forall h', exit_edge h' p q -> h = h';
+      no_exit_head : forall h p q, exit_edge h p q -> ~ loop_head q;
+      exit_pred_loop : forall h q qe e, exit_edge h qe e -> q --> e -> loop_contains h q;
+      no_self_loops : forall q p, edge q p = true -> q <> p;
+      root_no_pred : forall p, edge p root <> true
+    }.
+
+Hint Resolve loop_head_dom a_edge_incl a_edge_acyclic a_reachability.
+
+
+  Lemma ne_list_nlrcons: forall (A : Type) (l : ne_list A), exists (a : A) (l' : list A), l = l' >: a.
+  Proof.
+    induction l.
+    - exists a, nil. eauto.
+    - destructH. rewrite IHl. exists a0, (a :: l'). cbn. reflexivity.
+  Qed.
+  
+  Ltac destr_r x :=
+    let Q := fresh "Q" in
+    specialize (ne_list_nlrcons x) as Q;
+    let a := fresh "a" in
+    let l := fresh "l" in
+    destruct Q as [a [l Q]];
+    rewrite Q in *.
+  
+  Definition CPath `{redCFG} := Path edge.
+  Definition APath `{redCFG} := Path a_edge.
+  Infix "↪" := back_edge (at level 55).
+  Notation "p '-->*' q" := (exists π, CPath p q π) (at level 55, right associativity).
+  Notation "p '-a>*' q" := (exists π, APath p q π) (at level 55).
+
+Section cfg.
+  Context `{C : redCFG}.
+
+  Notation "p '-a>b' q" := (a_edge p q) (at level 55).
+  Notation "p '-a>' q" := (p -a>b q = true) (at level 55).
+  Notation "p '-->b' q" := (edge p q) (at level 55).
+  Notation "p '-->' q" := (p -->b q = true) (at level 55, right associativity).
+
+  (** abbreviation for CPath **)
+  Definition CPath' π := CPath (ne_back π) (ne_front π) π.
+
+  Lemma cpath_cpath' (* unused *)r p t
+        (Hpath : CPath r p t)
+    : CPath' t.
+  Proof.
+    unfold CPath'. eapply path_back in Hpath as Hback.
+    eapply path_front in Hpath as Hfront.
+    rewrite Hfront,Hback. assumption.
+  Qed.
+  
+  (*
+Local Ltac prove_spec :=
+  intros;
+  let tac :=
+      fun _ => lazymatch goal with
+              [ |- to_bool ?e = true <-> ?p] => destruct e; cbn; split; eauto ; intros; congruence
+            end
+  in
+  lazymatch goal with
+  | [ |- ?f _ _ _ = true <-> ?p ]
+    => unfold f; tac 0
+  | [ |- ?f _ _ = true <-> ?p ]
+    => unfold f; tac 0
+  | [ |- ?f _ = true <-> ?p ]
+    => unfold f; tac 0
+  | [ |- ?f = true <-> ?p ]
+    => unfold f; tac 0
+  end.*)
+
+  (** decidable properties on redCFG **)
+  
+  Global Instance Lab_dec : EqDec Lab eq.
+  Proof.
+    intros x y. destruct (decide_eq x y).
+    - left. rewrite e. reflexivity.
+    - right. eauto.
+  Qed.
+  
+  Instance loop_head_dec p : dec (loop_head p).
+    eauto.
+  Qed.
+
+  (* I could also prove that, but it is not trivial non-classical. *)  
+  Parameter loop_contains_dec : forall qh q, dec (loop_contains qh q).
+  Global Existing Instance loop_contains_dec.
+  
+  Hint Resolve loop_contains_dec.
+
+  Global Instance exit_edge_dec : forall h p q, dec (exit_edge h p q).
+  Proof.
+    eauto.
+  Qed.
+
+  Definition exiting (h p : Lab) : Prop :=
+    exists q, exit_edge h p q.
+
+  Definition exited (h q : Lab) : Prop :=
+    exists p, exit_edge h p q.
+
+  Global Instance exited_dec (h q : Lab) : dec (exited h q).
+  Proof.
+    eauto.
+  Qed.
+
+  Lemma back_edge_dec p q : dec (p ↪ q).
+  Proof.
+    unfold back_edge, back_edge_b, minus_edge.
+    destruct (edge p q), (a_edge p q);cbn;firstorder.
+  Qed.
+
+  Hint Resolve back_edge_dec.
+
+  (** Some basic facts **)
+  
+  Lemma reachability (q : Lab) : exists π : ne_list Lab, Path edge root q π.
+  Proof.
+    specialize (a_reachability q) as Hreach. destructH. exists π. eapply subgraph_path';eauto. 
+  Qed.
+  
+  Lemma back_edge_incl (p q : Lab) (Hback : p ↪ q) : edge p q = true.
+  Proof. 
+    unfold back_edge,back_edge_b in Hback. eapply minus_subgraph. eauto.
+  Qed.
+
+  Lemma acyclic_path_NoDup p q π
+        (Hπ : Path a_edge p q π)
+    : NoDup π.
+  Proof.
+    induction Hπ.
+    - econstructor;eauto. econstructor.
+    - cbn. econstructor;auto.
+      intro N. specialize a_edge_acyclic as Hacy. unfold acyclic in Hacy.
+      eapply path_from_elem in N;eauto. destructH. apply Hacy in N0;eauto.
+  Qed.
+  
+  (** about loops **)
+  
+  Lemma loop_contains_loop_head (qh q : Lab)
+    : loop_contains qh q -> loop_head qh.
+  Proof.
+    intro Q. unfold loop_head, loop_contains in *. destruct Q as [p [_ [Q _]]].
+    eexists; eauto.
+  Qed.
+
+  Lemma loop_contains_self h : loop_head h -> loop_contains h h.
+  Proof.
+    intros Hl. unfold loop_contains.
+    - unfold loop_head in Hl. destruct Hl. 
+      eapply loop_head_dom in H as Hdom.
+      eapply back_edge_incl in H as Hreach. specialize (a_reachability x) as Hreach'.
+      destructH.
+      eapply subgraph_path' in Hreach' as Hreach'';eauto using a_edge_incl.
+      eapply Hdom in Hreach''. eapply path_from_elem in Hreach''; eauto.
+      destructH; eauto.
+      eapply path_NoDup' in Hreach''0;eauto. 
+      destructH. exists x, π0. firstorder;eauto.
+      + eapply subgraph_path';eauto using a_edge_incl.
+      + eapply NoDup_rev in Hreach''3. eapply path_back in Hreach''2.
+        remember (rev π0) as l.
+        destruct l;cbn in *;eauto.
+        specialize (ne_list_nlrcons π0) as Heql'. destructH. subst π0. cbn in *. simpl_nl' Heql.
+        rewrite rev_rcons in Heql. inversion Heql;subst e l.
+        simpl_nl' Hreach''2. subst. inversion Hreach''3;subst. auto.
+  Qed.
+  
+End cfg.
