CFGinnermost.v
@@ -1,0 +1,396 @@
+Require Export CFGdeq.
+
+Section cfg.
+  Context `{C : redCFG}.
+  
+  Notation "p '-a>b' q" := (a_edge p q) (at level 55).
+  Notation "p '-a>' q" := (p -a>b q = true) (at level 55).
+  Notation "p '-->b' q" := (edge p q) (at level 55).
+  Notation "p '-->' q" := (p -->b q = true) (at level 55, right associativity).
+  
+  (** innermost_loops **)
+  
+  Definition innermost_loop h p : Prop := loop_contains h p /\ deq_loop h p.
+
+  Definition innermost_loop_strict (h p : Lab)
+    := loop_contains h p /\ h <> p /\ forall h', loop_contains h' p -> (loop_contains h' h \/ h' = p).
+  
+  Definition finType_sig_or_never (X : finType) (P : decPred X) : {x : X | P x} + {forall x : X, ~ P x}.
+  Proof.
+    remember (filter P (elem X)).
+    destruct l.
+    - right. intros ? ?. specialize (in_filter_iff P x (elem X)) as Hiff. rewrite <-Heql in Hiff.
+      cbn in Hiff. eapply Hiff. split;eauto.
+    - left. econstructor. specialize (in_filter_iff P e (elem X)) as Hiff.
+      rewrite <-Heql in Hiff. cbn in Hiff. eapply Hiff. eauto.
+  Qed.
+  
+  Definition ex_innermost_loop p
+    := finType_sig_or_never (DecPred (fun h => innermost_loop h p)).
+    
+  Definition ex_innermost_loop_strict (p : Lab)
+    : {h : Lab | innermost_loop_strict h p} + {forall h, ~ innermost_loop_strict h p}
+    := finType_sig_or_never (DecPred (fun h => innermost_loop_strict h p)).
+
+  Definition get_innermost_loop (p : Lab) : option Lab :=
+    match ex_innermost_loop p with
+    | inleft (exist _ h _) => Some h
+    | inright _ => None
+    end.
+
+  Definition get_innermost_loop_strict (p : Lab) : option Lab :=
+    match ex_innermost_loop_strict p with
+    | inleft (exist _ h _) => Some h
+    | inright _ => None
+    end.
+  
+  Definition get_innermost_loop_dep (p : Lab) : option {h : Lab | loop_contains h p} :=
+    match ex_innermost_loop p with
+    | inleft (exist _ h H) => Some (exist _ h (match H with
+                                              | conj Q _ => Q
+                                              end))
+    | inright _ => None
+    end.                    
+  
+  Definition get_innermost_loop_strict_dep (p : Lab) : option {h : Lab | loop_contains h p} :=
+    match ex_innermost_loop_strict p with
+    | inleft (exist _ h H) => Some (exist _ h (match H with
+                                              | conj Q _ => Q
+                                              end))
+    | inright _ => None
+    end.
+
+  Lemma innermost_loop_strict_unique (* unused *)(h h' p : Lab)
+        (H : innermost_loop_strict h p)
+        (Q : innermost_loop_strict h' p)
+    : h = h'.
+  Proof.
+    unfold innermost_loop_strict in *. do 2 destructH.
+    eapply H3 in Q0. destruct Q0;[|contradiction].
+    eapply Q3 in H0. destruct H0;[|contradiction].
+    eapply loop_contains_Antisymmetric;auto.
+  Qed.
+
+  Definition LPath := Path (fun h p => decision (innermost_loop_strict h p)).
+  
+  (** StrictPrefix **)
+
+  Definition StrictPrefix' := 
+    fun (A : Type) (l l' : ne_list A) => exists a : A, Prefix (a :<: l) l'.
+
+  Lemma prefix_strictPrefix:
+    forall (e : Lab) (x ϕ : ne_list Lab), Prefix ϕ x -> StrictPrefix' ϕ (e :<: x).
+  Proof.
+    intros e x ϕ Hϕ1.
+    unfold StrictPrefix'. cbn.
+    revert dependent e.
+    induction Hϕ1; intros.
+    - exists e; econstructor.
+    - specialize(IHHϕ1 a). destructH. exists a0. econstructor. auto.
+  Qed.
+
+  Lemma StrictPrefix_well_founded (A : Type) : well_founded (@StrictPrefix' A).
+  Proof.
+    unfold well_founded.
+    intros. 
+    induction a.
+    - econstructor. intros. unfold StrictPrefix' in *. destructH. inversion H;[congruence'|]. inversion H2.
+    - constructor. intros.
+      unfold StrictPrefix' in H.
+      destructH. cbn in *. inversion H;subst.
+      + eapply ne_to_list_inj in H3. subst. auto.
+      + eapply IHa. unfold StrictPrefix'. exists a1. cbn. auto.
+  Qed.
+  
+  Lemma find_some_strong (A : Type) `{Q:EqDec A eq} (f : A -> bool) (l : list A) (x : A) (Hnd : NoDup l)
+    : find f l = Some x -> x ∈ l /\ f x = true /\ forall y, y ≻* x | l -> f y = true -> x = y.
+  Proof.
+    repeat split. 1,2: eapply find_some in H; firstorder.
+    revert dependent x.
+    induction l;intros.
+    - inversion H0.
+    - cbn in H.
+      destruct (f a) eqn:E.
+      + inversion H; subst. inversion H0;subst;auto.
+        inversion Hnd; subst. exfalso; contradict H5. eapply splinter_incl;[eapply H4|]. firstorder 0.
+      + destruct (a == y);[rewrite e in E;congruence|].
+        inversion Hnd; subst. eapply IHl;eauto. inversion H0;subst;auto. congruence.
+  Qed.
+
+  (** LPath **)
+  
+  Lemma loop_LPath_helper p h π
+        (Hpath : Path a_edge root p (p :<: π))
+        (Hloop : loop_contains h p)
+        (Hin : h ∈ π)
+        (Hnolo : forall q : Lab, q ≻* h | π -> toBool _ (D:=decision (loop_contains q p)) = true -> h = q)
+    : (forall h' : Lab, loop_contains h' p -> loop_contains h' h \/ h' = p).
+  Proof.
+    intros. eapply loop_contains_either in H as H';[|apply Hloop].
+    destruct H';[|left;auto].
+    decide (h' = p);[right;auto|]. 
+    specialize (Hnolo h'). exploit Hnolo.
+    - eapply subgraph_path' in Hpath;eauto using a_edge_incl.
+      eapply loop_contains_splinter in Hpath;eauto.
+      cbn in Hpath. inversion Hpath;subst;auto. inversion H2;subst;contradiction.
+    - decide (loop_contains h' p); cbn in *;[congruence|contradiction].
+    - subst. left. eapply loop_contains_self. eapply loop_contains_loop_head;eauto.
+  Qed.
+  
+  Lemma loop_LPath h p
+        (Hloop : loop_contains h p)
+    : exists π, LPath h p π.
+  Proof.
+    specialize (a_reachability p) as Hreach.
+    destructH. revert dependent p. revert dependent π.
+    specialize (well_founded_ind (R:=(@StrictPrefix' Lab)) (@StrictPrefix_well_founded Lab)
+                                 (fun π : ne_list Lab => forall p, loop_contains h p
+                                                           -> Path a_edge root p π
+                                                           -> exists (π0 : ne_list Lab), LPath h p π0))
+      as WFind.
+    eapply WFind.
+    intros;clear WFind.
+    destruct x.
+    - inversion H1; subst p a e.
+      eapply root_loop_root in H0. subst. repeat econstructor.
+    - remember (find (fun h' => decision (loop_contains h' p)) x) as S.
+      destruct S; symmetry in HeqS.
+      + eapply find_some_strong in HeqS. destructH. decide (loop_contains e0 p);cbn in *;[|congruence].
+        inversion H1;subst.
+        decide (h = e).
+        { subst;eexists;econstructor. }
+        specialize (path_to_elem _ a_edge _ _ e0 x H6 HeqS0) as [ϕ [Hϕ0 Hϕ1]].
+        specialize (H ϕ). exploit' H.
+        { cbn. clear - Hϕ1.
+          eapply prefix_strictPrefix;auto.
+        } 
+        specialize (H e0). exploit H.
+        { clear - l H0 n HeqS0 HeqS3 H1.
+          decide (e0 = h);[subst;eapply loop_contains_self;unfold loop_contains in H0;firstorder|].
+          eapply loop_contains_either in H0 as H0'; eauto.
+          destruct H0';[exfalso|auto].
+          eapply (loop_LPath_helper) in HeqS3;auto. 2:exact H0. destruct HeqS3;[|contradiction].
+          eapply loop_contains_Antisymmetric in H. exploit H. contradiction.
+        } 
+        destructH.        
+        exists (e :<: π0).
+        econstructor;cycle 1.
+        * instantiate (1:=e0). decide (innermost_loop_strict e0 e);cbn;[auto|exfalso;contradict n0].
+          unfold innermost_loop_strict. split;auto. split.
+          -- eapply acyclic_path_NoDup in H1. clear - HeqS0 H1. inversion H1; subst.
+             contradict H2. subst. auto.
+          -- eapply loop_LPath_helper;eauto.
+        * auto.
+        * auto.
+        * inversion H1;subst. eapply acyclic_path_NoDup; eauto.
+      + decide (h = e); subst.
+        { inversion H1. subst. repeat econstructor. }
+        eapply find_none in HeqS;cycle 1.
+        * instantiate (1:=h).
+          enough (h ∈ (e :<: x)) as Hex.
+          { destruct Hex;[symmetry in H2;contradiction|auto]. }
+          eapply dom_dom_acyclic;eauto. eapply dom_loop;auto.
+        * exfalso. decide (loop_contains h p); cbn in *; [congruence|contradiction].
+  Qed.    
+  
+  Lemma loop_contains_innermost (h p : Lab)
+        (Hloop : loop_contains h p)
+    : exists h', innermost_loop h' p.
+  Proof.
+    unfold innermost_loop.
+    eapply loop_LPath in Hloop as Hloop'. destructH.
+    decide (loop_head p).
+    + exists p. split;eauto using loop_contains_self. unfold deq_loop; firstorder.
+    + inversion Hloop'. subst.
+      * exists p. split;eauto using loop_contains_self. unfold deq_loop; firstorder.
+      * subst. exists b.
+        decide (innermost_loop_strict b p);cbn in *;[|congruence]. unfold innermost_loop_strict in i.
+        clear - i n. destructH. unfold deq_loop.
+        split;auto. intros. exploit i3. destruct i3;auto.
+        subst. eapply loop_contains_loop_head in H. contradiction.
+  Qed.
+
+  Lemma loop_contains_innermost_strict (h p : Lab)
+        (Hloop : loop_contains h p)
+        (Hneq : h <> p)
+    : exists h', innermost_loop_strict h' p.
+  Proof.
+    eapply loop_LPath in Hloop as Hloop'. destructH.
+    inversion Hloop';subst;eauto;[contradiction|].
+    exists b. decide (innermost_loop_strict b p);cbn in *;[auto|congruence].
+  Qed.
+  
+  Lemma get_innermost_loop_spec
+    : forall p : Lab,
+      match get_innermost_loop p with
+      | Some h => innermost_loop h p
+      | None => forall h' : Lab, loop_contains h' p -> False
+      end.
+  Proof.
+    unfold get_innermost_loop.
+    intro. destruct (ex_innermost_loop p).
+    - destruct s;eauto.
+    - cbn in n. unfold innermost_loop in n. intros.
+      eapply loop_contains_innermost in H. clear h'. destructH.
+      specialize (n h'). eapply dec_DM_and in n;eauto.
+      destruct n;unfold innermost_loop in H;firstorder.
+  Qed.
+  
+  Lemma get_innermost_loop_dep_spec
+    : forall p : Lab,
+      match get_innermost_loop_dep p with
+      | Some (exist _ h _) => innermost_loop h p
+      | None => forall h' : Lab, loop_contains h' p -> False
+      end.
+  Proof.
+    unfold get_innermost_loop_dep.
+    intro. destruct (ex_innermost_loop p).
+    - destruct s;eauto.
+    - cbn in n. unfold innermost_loop in n. intros.
+      eapply loop_contains_innermost in H. clear h'. destructH.
+      specialize (n h'). eapply dec_DM_and in n;eauto.
+      destruct n;unfold innermost_loop in H;firstorder.
+  Qed.
+
+  Lemma get_innermost_loop_strict_spec (* unused *)(p : Lab)
+    : match get_innermost_loop_strict p with
+      | Some h => innermost_loop_strict h p
+      | None => forall h', loop_contains h' p -> h' = p
+      end.
+  Proof.
+    unfold get_innermost_loop_strict.
+    destruct (ex_innermost_loop_strict p); cbn.
+    - destruct s. eauto.
+    - intros. 
+      decide (h' = p);[eauto|].
+      eapply loop_contains_innermost_strict in H;eauto.
+      destructH. specialize (n h'0); contradiction.
+  Qed.
+  
+  Lemma get_innermost_loop_strict_dep_spec (* unused *)(p : Lab)
+    : match get_innermost_loop_strict_dep p with
+      | Some (exist _ h H) => innermost_loop_strict h p
+      | None => forall h', loop_contains h' p -> h' = p
+      end.
+  Proof.
+    unfold get_innermost_loop_strict_dep.
+    destruct (ex_innermost_loop_strict p); cbn.
+    - destruct s. eauto.
+    - intros. 
+      decide (h' = p);[eauto|].
+      eapply loop_contains_innermost_strict in H;eauto.
+      destructH. specialize (n h'0); contradiction.
+  Qed.
+  
+  Lemma deq_loop_trans p q r
+        (H1 : deq_loop p q)
+        (H2 : deq_loop q r)
+    : deq_loop p r.
+  Proof.
+    unfold deq_loop in *. intros. eapply H1,H2;eauto.
+  Qed.
+
+  Program Instance deq_loop_PreOrder : PreOrder deq_loop.
+  Next Obligation.
+    unfold Reflexive. eapply deq_loop_refl.
+  Qed.
+  Next Obligation.
+    unfold Transitive; eapply deq_loop_trans.
+  Qed.
+
+  Lemma loop_contains_deq_loop h p
+        (Hloop : loop_contains h p)
+    : deq_loop p h.
+  Proof.
+    unfold deq_loop. intros. eapply loop_contains_trans;eauto.
+  Qed.
+
+  Lemma innermost_loop_deq_loop (* unused *)h p q
+        (Hinner : innermost_loop h p)
+        (Hloop : loop_contains h q)
+    : deq_loop q p.
+  Proof.
+    unfold innermost_loop in Hinner. destructH.
+    eapply deq_loop_trans;eauto.
+    eapply loop_contains_deq_loop;eauto.
+  Qed.
+
+  (** preds **)
+
+  Definition preds `{redCFG Lab edge} p : list Lab := filter (decPred_bool (fun q => edge q p)) (elem Lab). 
+
+  Lemma preds_in_same_loop h p q
+        (Hl : loop_contains h p)
+        (Hneq : h <> p)
+        (Hedge : q --> p)
+    : loop_contains h q.
+  Proof.
+    unfold loop_contains in Hl.
+    destructH.
+    eapply path_rcons in Hl2 as Hl2';eauto.
+    exists p0, (π :>: q). repeat (split;eauto).
+    simpl_nl. rewrite rev_rcons. cbn. eapply nin_tl_iff in Hl3;auto.
+    destruct Hl3 as [Hl3|Hl3];[contradict Hl3;eapply in_rev;auto|eapply path_back in Hl2;subst;auto].
+  Qed.
+
+  Lemma deq_loop_exited h qe e
+        (Hexit : exit_edge h qe e)
+    : deq_loop qe e.
+  Proof.
+    eapply no_exit_head in Hexit as Hneh.
+    unfold exit_edge in *. destructH.
+    unfold deq_loop. intros. 
+    eapply preds_in_same_loop in H;eauto.
+    intro N. eapply loop_contains_loop_head in H. subst. contradiction.
+  Qed.
+  
+  Lemma deq_loop_exiting h qe e
+        (Hexit : exit_edge h qe e)
+    : deq_loop h qe.
+  Proof.
+    unfold deq_loop;intros. copy Hexit Hexit'.
+    unfold exit_edge in Hexit. destructH. eapply loop_contains_either in Hexit0;eauto.
+    destruct Hexit0;[auto|].
+    enough (h = h0) by (subst;eauto using loop_contains_self,loop_contains_loop_head).
+    eapply single_exit;eauto.
+    unfold exit_edge. repeat (split;eauto).
+    contradict Hexit2. eapply loop_contains_trans;eauto.
+  Qed.
+
+  Definition get_innermost_loop' p
+    := match get_innermost_loop p with
+       | Some h => h
+       | None => root
+       end.
+
+  Lemma deq_loop_innermost' (p : Lab)
+    : deq_loop (get_innermost_loop' p) p.
+  Proof.
+    remember (get_innermost_loop' p) as h.
+    specialize (get_innermost_loop_spec p) as Hspec.
+    unfold get_innermost_loop' in Heqh.
+    destruct (get_innermost_loop p).
+    - subst. unfold innermost_loop in Hspec. subst. destructH; auto.
+    - subst. unfold deq_loop. intros. exfalso; eauto.
+  Qed.
+  Definition innermost_loop' (* unused *)`{redCFG} (h p : Lab) := (loop_contains h p \/ h = root) /\ deq_loop h p.
+
+  Definition get_innermost_loop_strict' p
+    := match get_innermost_loop_strict p with
+       | Some h => h
+       | None => root
+       end.
+
+  Lemma eq_loop_innermost h p q
+        (Heq : eq_loop p q)
+        (Hinner : innermost_loop h p)
+    : innermost_loop h q.
+  Proof.
+    unfold innermost_loop in *.
+    destructH.
+    split;[eapply Heq in Hinner0;auto|]. 
+    unfold eq_loop in Heq. destructH.
+    eapply deq_loop_trans;eauto.
+  Qed.
+
+End cfg.
