SimplDec.v
@@ -1,0 +1,51 @@
+Require Export FinTypes.
+
+
+Lemma dec_DM_and_iff (X Y : Prop) : dec X -> ~ (X /\ Y) <-> ~ X \/ ~ Y.
+  split;[now eapply dec_DM_and|firstorder].
+Qed.
+Lemma dec_DM_and_iff' (* unused *)(X Y : Prop) : dec Y -> ~ (X /\ Y) <-> ~ X \/ ~ Y.
+  split;[now eapply dec_DM_and'|firstorder].
+Qed.
+Lemma dec_DN_iff (* unused *)(X : Prop) : dec X -> ~ ~ X <-> X.
+  split;[now eapply dec_DN|firstorder].
+Qed.
+Lemma dec_DM_impl_iff (X Y : Prop) : dec X -> dec Y -> ~ (X -> Y) <-> X /\ ~ Y.
+  split;[now eapply dec_DM_impl|firstorder].
+Qed.
+
+Ltac simpl_dec' H :=
+  (first [(setoid_rewrite (DM_notAll _) in H;eauto)|
+          (setoid_rewrite (dec_DM_and_iff _ _) in H;eauto)|
+          (setoid_rewrite (dec_DM_and_iff' _ _) in H;eauto)|
+          setoid_rewrite DM_not_exists in H|
+          setoid_rewrite DM_or in H|
+          (setoid_rewrite (dec_DN_iff _) in H;eauto)|
+          (setoid_rewrite (dec_DM_impl_iff _ _) in H;eauto)]).
+Ltac simpl_dec :=
+  (try (setoid_rewrite DM_notAll;[|eauto]);
+   try (setoid_rewrite (dec_DM_and_iff _ _);[|eauto]);
+   try (setoid_rewrite (dec_DM_and_iff' _ _);[|eauto]);
+   try setoid_rewrite DM_not_exists;
+   try setoid_rewrite DM_or;
+   try (setoid_rewrite (dec_DN_iff _);[|eauto]);
+   try (setoid_rewrite (dec_DM_impl_iff _ _);eauto)).
+
+(*Ltac collapse H :=
+  lazymatch type of H with
+  | ?a /\ ?b => let H1 := fresh "H" in
+              let H2 := fresh "H" in
+              destruct H as [H1 H2];
+              collapse H1;
+              collapse H2
+  | ?a \/ ?b => destruct H as [H|H]; collapse H
+  | ~ ?x => simpl_dec' H; collapse H
+  | _ => idtac
+  end.*)
+
+
+
+Goal forall (X : finType) (P Q : X -> Prop), (forall x, dec (P x)) -> (forall x, dec (Q x)) -> ~ (forall x, P x \/ Q x) -> False.
+  intros. (*setoid_rewrite (DM_notAll _) in H.*) (*evar (forall x, P x \/ Q x).*)
+  simpl_dec' H.
+Abort.
